added support for interface files (needs to be tightened up a bit); tc type-checks itself in about 1 minute (without queries, of course)

src/absyn/syntax.fs
@@ -224,6 +224,7 @@ type modul = {
   name: lident;
   declarations: sigelts;
   exports: sigelts;
+  is_interface:bool
 }
 
 (*********************************************************************************)
