src/basic/util.fs
@@ -60,6 +60,7 @@ let string_of_float i = string_of_float i
 let string_of_char  (i:char) = spr "%A" i
 let string_of_bytes (i:byte[]) = string_of_unicode i
 let starts_with (s1:string) (s2:string) = s1.StartsWith(s2)
+let ends_with (s1:string) (s2:string) = s1.EndsWith(s2)
 let char_at (s:string) (i:int) : char = s.[i]
 
 let iof = int_of_float
