src/parser/desugar.fsi
@@ -1,0 +1,36 @@
+﻿(*
+  Copyright 2008-2014 Nikhil Swamy and Microsoft Research
+
+  Licensed under the Apache License, Version 2.0 (the "License");
+  you may not use this file except in compliance with the License.
+  You may obtain a copy of the License at
+
+  http://www.apache.org/licenses/LICENSE-2.0
+
+  Unless required by applicable law or agreed to in writing, software
+  distributed under the License is distributed on an "AS IS" BASIS,
+  WITHOUT WARRANTIES OR CONDITIONS OF ANY KIND, either express or implied.
+  See the License for the specific language governing permissions and
+  limitations under the License.
+*)
+#light "off"
+module Microsoft.FStar.Parser.Desugar
+
+open Microsoft.FStar
+open Microsoft.FStar.Parser
+open Microsoft.FStar.Range
+open Microsoft.FStar.Parser.AST
+open Microsoft.FStar.Parser.DesugarEnv
+open Microsoft.FStar.Absyn
+open Microsoft.FStar.Absyn.Syntax
+open Microsoft.FStar.Absyn.Util
+open Microsoft.FStar.Util
+
+val desugar_file: env -> file -> env * list<modul>
+
+(* private *) val desugar_modul : env -> AST.modul -> env * Syntax.modul
+(* private *) val desugar_kind_abbrev : range -> env -> ident -> list<binder> -> term -> env * kind_abbrev
+(* private *) val mk_data_ops : env -> sigelt -> list<sigelt>
+(* private *) val close : env -> term -> term
+(* private *) val op_as_tylid : range -> string -> option<lident>
+(* private *) val op_as_vlid : env -> int -> range -> string -> option<lident>
