src/parser/dsenv.fsi
@@ -1,0 +1,106 @@
+﻿(*
+   Copyright 2008-2014 Nikhil Swamy and Microsoft Research
+
+   Licensed under the Apache License, Version 2.0 (the "License");
+   you may not use this file except in compliance with the License.
+   You may obtain a copy of the License at
+
+       http://www.apache.org/licenses/LICENSE-2.0
+
+   Unless required by applicable law or agreed to in writing, software
+   distributed under the License is distributed on an "AS IS" BASIS,
+   WITHOUT WARRANTIES OR CONDITIONS OF ANY KIND, either express or implied.
+   See the License for the specific language governing permissions and
+   limitations under the License.
+*)
+#light "off"
+// (c) Microsoft Corporation. All rights reserved
+
+module Microsoft.FStar.Parser.DesugarEnv
+
+
+open Microsoft.FStar
+open Microsoft.FStar.Util
+open Microsoft.FStar.Absyn
+open Microsoft.FStar.Absyn.Syntax
+open Microsoft.FStar.Absyn.Util
+open Microsoft.FStar.Absyn.Const
+open Microsoft.FStar.Parser
+    
+type binding = 
+  | Binding_typ_var of ident
+  | Binding_var of ident
+  | Binding_let of lident
+  | Binding_tycon of lident
+
+type kind_abbrev = lident * list<either<btvdef, bvvdef>> * Syntax.knd
+type env = {
+  curmodule: option<lident>;
+  modules:list<(lident * modul)>;  (* previously desugared modules *)
+  open_namespaces: list<lident>; (* fully qualified names, in order of precedence *)
+  sigaccum:sigelts;              (* type declarations being accumulated for the current module *)
+  localbindings:list<(either<btvdef,bvvdef> * binding)>;  (* local name bindings for name resolution, paired with an env-generated unique name *)
+  kind_abbrevs:list<kind_abbrev>;
+  recbindings:list<binding>;     (* names bound by recursive type and top-level let-bindings definitions only *)
+  phase:AST.level;
+  sigmap: Util.smap<(sigelt * bool)>; (* bool indicates that this was declared in an interface file *)
+  effect_names:list<lident>;
+  default_result_effect:typ -> Range.range -> comp;
+  interf:bool
+}
+
+type record = {
+  typename: lident;
+  constrname: lident;
+  parms: list<tparam>;
+  fields: list<(fieldname * typ)>
+}
+
+val fail_or: (lident -> option<'a>) -> lident -> 'a
+val fail_or2: (ident -> option<'a>) -> ident -> 'a
+
+val qualify: env -> ident -> lident
+val qualify_lid: env -> lident -> lident
+
+val empty_env: unit -> env
+val total: env -> env
+val ml: env -> env
+
+val try_lookup_typ_var: env -> ident -> option<typ>
+val resolve_in_open_namespaces: env -> lident -> (lident -> option<'a>) -> option<'a>
+val try_lookup_typ_name: env -> lident -> option<typ>
+val is_effect_name: env -> lident -> bool
+val try_resolve_typ_abbrev: env -> lident -> option<typ>
+val try_lookup_id: env -> ident -> option<exp>
+
+val try_lookup_lid: env -> lident -> option<exp>
+val try_lookup_datacon: env -> lident -> option<var<typ>>
+val try_lookup_record_by_field_name: env -> lident -> option<(record * lident)>
+
+val qualify_field_to_record: env -> record -> lident -> option<lident>
+val find_kind_abbrev: env -> lident -> option<kind_abbrev>
+val is_kind_abbrev: env -> lident -> bool
+val push_kind_abbrev: env -> kind_abbrev -> env
+val push_bvvdef: env -> bvvdef -> env
+val push_btvdef: env -> btvdef -> env
+val push_local_binding: env -> binding -> env * either<btvdef, bvvdef>
+val push_local_vbinding: env -> ident -> env * bvvdef
+val push_local_tbinding: env -> ident -> env * btvdef
+val push_rec_binding: env -> binding -> env
+val push_sigelt: env -> sigelt -> env
+val push_namespace: env -> lident -> env
+val is_type_lid: env -> lident -> bool
+
+val finish_module_or_interface: env -> modul -> env
+val prepare_module_or_interface: bool -> env -> lident -> env
+val enter_monad_scope: env -> ident -> env
+val exit_monad_scope: env -> env -> env
+
+(* private *) val unmangleOpName: ident -> option<lident>
+(* private *) val try_lookup_lid': bool -> bool -> env -> lident -> option<exp>
+(* private *) val extract_record: env -> sigelt -> unit
+(* private *) val unique_name: bool -> bool -> env -> lident -> bool
+(* private *) val unique_typ_name: env -> lident -> bool
+(* private *) val unique:  bool -> bool -> env -> lident -> bool
+(* private *) val check_admits:  env -> unit
+(* private *) val finish:  env -> modul -> env
